test: moved most of the testing infrastructure to the `TestingLib`
+ moved Taint Tracking to separate file with parametrized module

TestingLib.v
@@ -15,7 +15,7 @@ Require Export ExtLib.Structures.Monads.
 Require Import ExtLib.Data.List.
 Import MonadNotation.
 From Stdlib Require Import String.
-From SECF Require Import ListMaps MapsFunctor MiniCET.
+From SECF Require Import ListMaps MapsFunctor MiniCET Utils TaintTrackingMiniCET.
 Require Import Stdlib.Classes.EquivDec.
 
 (** ** Type system for cryptographic constant-time programming *)
@@ -452,3 +452,859 @@ Fixpoint max n m := match n, m with
                    | _, 0 => n
                    | S n', S m' => S (max n' m')
                    end.
+
+
+Module MCC := MiniCETCommon(ListTotalMap).
+Import MCC.
+
+(*! Section testing_ETE *)
+
+(** Type system for soundenss *)
+
+Inductive ty : Type := | TNum | TPtr.
+
+Derive (Arbitrary, Shrink) for ty.
+Derive Show for ty.
+
+Definition ty_eqb (x y: ty) := match x, y with
+                               | TNum, TNum | TPtr, TPtr => true
+                               | _, _ => false
+                               end.
+
+Definition rctx := ListTotalMap.t ty.
+Definition tmem := list ty.
+
+Fixpoint ty_of_exp (c : rctx) (e : exp) : ty :=
+  match e with
+  | ANum _ => TNum
+  | AId x => c ! x
+  | ABin _ _ _ => TNum
+  (* Here we assume that "e" is well-typed and infer the type by the second branch of "ACTIf"  *)
+  | ACTIf _ _ x => ty_of_exp c x
+  | FPtr _ => TPtr
+end.
+
+Definition filter_vars_by_ty (t: ty) (c: rctx) : list string :=
+  filter (fun x => ty_eqb (c ! x) t) (map_dom (snd c)).
+
+Definition is_ptr (c : rctx) (var : string) :=
+  match c ! var with
+  | TPtr => true
+  | _ => false
+  end.
+
+(* predicate for fold *)
+Definition is_br_or_call (i : inst) :=
+  match i with
+  | <{{branch _ to _}}> | <{{call _}}> => true
+  | _                                  => false
+  end.
+
+(** Well-formed Program Generator *)
+
+(* This auxiliary function, given a program length, generates the length of procedures in this program, counted in blocks.
+   It therefore partitions the program in procedures. *)
+Fixpoint _gen_partition (fuel program_length: nat) : G (list nat) :=
+  match fuel with
+  | 0 => ret [program_length]
+  | S fuel' =>
+      match program_length with
+      | O => ret []
+      | S O => ret [1]
+      | S (S program_length') => (k <- choose(1, program_length - 1);;
+                     rest <- _gen_partition fuel' (program_length - k);;
+                     ret (k :: rest))
+      end
+  end.
+
+Definition gen_partition (pl: nat): G (list nat) := _gen_partition pl pl.
+
+Fixpoint proc_hd (pst: list nat) : list nat :=
+  match pst with
+  | [] => []
+  | hd :: tl => 0 :: map (fun x => x + hd) (proc_hd tl)
+  end.
+
+Compute (proc_hd [3; 3; 1; 1]).
+(* = <{{ i[ 0; 3; 6; 7] }}> *)
+
+Definition gen_callable (pl : nat) : G (list nat) :=
+  pst <- gen_partition pl ;; ret (proc_hd pst).
+
+Definition gen_vars (len: nat) : G (list string) :=
+  vectorOf len arbitrary.
+
+Sample (gen_vars 5).
+
+Definition ex_vars : list string :=
+  ["X0"%string; "X1"%string; "X2"%string; "X3"%string; "X4"%string].
+
+Fixpoint remove_dupes {a:Type} (eqb:a->a->bool) (t : list a) : list a :=
+  match t with
+  | [] => []
+  | x :: xs => if existsb (eqb x) xs
+               then      remove_dupes eqb xs
+               else x :: remove_dupes eqb xs
+  end.
+
+#[export] Instance genTMem `{Gen ty} : Gen tmem :=
+  {arbitrary := t <- arbitrary;;
+                tm <- arbitrary;;
+                ret (t :: tm) }.
+
+(* Similar to the previous expressions generators, we now generate the well-typed leaves, which
+  differentiate between different types of values in the program. *)
+Definition gen_exp_leaf_wt (t: ty) (c: rctx) (pst: list nat) : G exp :=
+  match t with
+  | TNum =>
+      oneOf (liftM ANum arbitrary ;;;
+               (let not_ptrs := filter (fun x => negb (is_ptr c x)) (map_dom (snd c)) in
+                if seq.nilp not_ptrs then [] else
+                  [liftM AId (elems_ "X0"%string not_ptrs)] ) )
+  | _ =>
+      oneOf (liftM FPtr (elems_ 0 (proc_hd pst));;;
+               (let ptrs := filter (fun x => (is_ptr c x)) (map_dom (snd c)) in
+                if seq.nilp ptrs then [] else
+                  [liftM AId (elems_ "X0"%string ptrs)] ) )
+  end.
+
+Fixpoint gen_exp_no_ptr_wt (sz : nat) (c : rctx) (pst: list nat) : G exp :=
+  match sz with
+  | O => gen_exp_leaf_wt TNum c []
+  | S sz' =>
+      freq [ (2, gen_exp_leaf_wt TNum c []);
+             (sz, eitherOf
+                    (liftM3 ABin arbitrary (gen_exp_no_ptr_wt sz' c pst) (gen_exp_no_ptr_wt sz' c pst))
+                    (liftM2 (ABin BinEq) (gen_exp_leaf_wt TPtr c pst)  (gen_exp_leaf_wt TPtr c pst)));
+             (sz, liftM3 ACTIf (gen_exp_no_ptr_wt sz' c pst) (gen_exp_no_ptr_wt sz' c pst) (gen_exp_no_ptr_wt sz' c pst))
+          ]
+  end
+with gen_exp_ptr_wt (sz : nat) (c : rctx) (pst: list nat) : G exp :=
+  match sz with
+  | O => gen_exp_leaf_wt TPtr c pst
+  | S sz' => 
+      freq [ (2, gen_exp_leaf_wt TPtr c pst);
+             (sz, liftM3 ACTIf (gen_exp_no_ptr_wt sz' c pst) (gen_exp_ptr_wt sz' c pst) (gen_exp_ptr_wt sz' c pst))
+          ]
+  end.
+
+Fixpoint gen_exp_wt (sz: nat) (c: rctx) (pst: list nat) : G exp :=
+  match sz with 
+  | O =>
+      t <- arbitrary;;
+      gen_exp_leaf_wt t c pst
+  | S sz' => 
+      freq [
+          (2, t <- arbitrary;; gen_exp_leaf_wt t c pst);
+          (sz, binop <- arbitrary;; match binop with
+                | BinEq => eitherOf
+                    (liftM2 (ABin BinEq) (gen_exp_no_ptr_wt sz' c pst) (gen_exp_no_ptr_wt sz' c pst))
+                    (liftM2 (ABin BinEq) (gen_exp_leaf_wt TPtr c pst) (gen_exp_leaf_wt TPtr c pst))
+                | _ => liftM2 (ABin binop) (gen_exp_no_ptr_wt sz' c pst) (gen_exp_no_ptr_wt sz' c pst)
+              end);
+             (sz, liftM3 ACTIf (gen_exp_no_ptr_wt sz' c pst) (gen_exp_wt sz' c pst) (gen_exp_wt sz' c pst))
+          ]
+  end.
+
+Fixpoint gen_exp_ty_wt (t: ty) (sz: nat) (c: rctx) (pst: list nat) : G exp :=
+  match t with
+  | TNum => gen_exp_no_ptr_wt sz c pst
+  | TPtr => gen_exp_ptr_wt sz c pst
+  end.
+
+Definition gen_val_wt (t: ty) (pst: list nat) : G val :=
+  match t with
+  | TNum => liftM N arbitrary
+  | TPtr => match (proc_hd pst) with
+           | [] => ret (FP 0)
+           | p::pst' => liftM FP (elems_ p (p::pst'))
+           end
+  end.
+
+Definition gen_reg_wt (c: rctx) (pst: list nat) : G reg :=
+  let wt_vars := snd c in
+  let gen_binds := mapGen (fun '(name, t) =>  (v <- gen_val_wt t pst;; ret (name, v))) wt_vars in
+  default_val <- gen_val_wt (fst c) pst;;
+  b <- gen_binds;;
+  ret (default_val, b).
+
+Definition wt_exp_is_defined := (forAll arbitrary (fun (c : rctx) =>
+            forAll (gen_reg_wt c [3; 3; 1; 1]) (fun (state: reg) =>
+            forAll (gen_exp_wt 4 c [3; 3; 1; 1]) (fun (exp : exp) =>
+            implication (is_defined (eval state exp)) true)))).
+(*! QuickChick wt_exp_is_defined. *)
+
+Definition gen_asgn_wt (t: ty) (c: rctx) (pst: list nat) : G inst :=
+  let tlst := filter (fun '(_, t') => ty_eqb t t') (snd c) in
+  let vars := map_dom tlst in
+  if seq.nilp vars
+  then ret <{ skip }>
+  else
+    x <- elems_ "X0"%string vars;;
+    a <- gen_exp_ty_wt t 1 c pst;;
+    ret <{ x := a }>.
+
+Definition gen_branch_wt (c: rctx) (pl: nat) (pst: list nat) (default : nat) : G inst :=
+  let vars := (map_dom (snd c)) in
+  let jlst := (list_minus (seq 0 pl) (proc_hd pst)) in
+  e <- gen_exp_ty_wt TNum 1 c pst;;
+  l <- elems_ default jlst;; (* 0 is unreachable *)
+  ret <{ branch e to l }>.
+
+Definition gen_jump_wt (pl: nat) (pst: list nat) (default : nat) : G inst :=
+  l <- elems_ default (list_minus (seq 0 pl) (proc_hd pst));; (* 0 is unreachable *)
+  ret <{ jump l }>.
+
+Definition filter_typed {A : Type} (t : ty) (l : list (A * ty)): list A := 
+  map fst (filter (fun '(_, t') => ty_eqb t t') l).
+
+Notation " 'elems' ( h ;;; tl )" := (elems_ h (cons h tl)) 
+  (at level 1, no associativity) : qc_scope.
+
+Definition gen_load_wt (t: ty) (c: rctx) (tm: tmem) (pl: nat) (pst: list nat) : G inst :=
+  let vars := filter_typed t (snd c) in
+  sz <- choose(1, 3);;
+  exp <- gen_exp_ty_wt TNum sz c pst;;
+  match vars with
+  | h :: tl =>
+    x <- elems ( h ;;; tl);;
+    ret <{ x <- load[exp] }>
+  | _ => ret <{ skip }>
+  end.
+
+Definition gen_store_wt (c: rctx) (tm: tmem) (pl: nat) (pst: list nat) : G inst :=
+  match tm with
+  | h :: tl =>
+    t <- elems (h ;;; tl);;
+    e1 <- gen_exp_ty_wt TNum 1 c pst;;
+    e2 <- gen_exp_ty_wt t 1 c pst;;
+    ret <{ store[e1] <- e2 }>
+  | _ => ret <{ skip }>
+  end.
+
+Definition compose_load_store_guard (t : ty) (id_exp : exp) (mem : tmem) : exp :=
+  let indices := seq 0 (Datatypes.length mem) in
+  let idx := filter_typed t (combine indices mem) in
+  let tc := fold_left 
+            (fun acc x => BOr x acc)
+            (map (fun id => <{{ id_exp = ANum id }}>) idx)
+            <{{ false }}> in
+  let mem_sz := ANum (Datatypes.length mem) in
+  let guardc := BLt id_exp mem_sz in
+  BAnd tc guardc. 
+Eval compute in (compose_load_store_guard TNum <{ AId "X0"%string }> [TNum ; TPtr; TNum ]).
+
+Definition transform_load_store_inst (c : rctx) (mem : tmem) (acc : list inst) (i : inst) : M (bool * list inst) :=
+  match i with
+  | <{{ x <- load[e] }}> =>
+      let t := t_apply c x in
+      merge <- add_block_M acc;;
+      new <- add_block_M <{{ i[ x <- load[e]; jump merge] }}>;;
+      ret (true, <{{ i[branch (compose_load_store_guard t e mem) to new; jump merge] }}>)
+  | <{{ store[e] <- e1 }}> =>
+      merge <- add_block_M acc;;
+      new <- add_block_M <{{ i[store[e] <- e1; jump merge] }}>;;
+      ret (true, <{{ i[branch (compose_load_store_guard (ty_of_exp c e1) e mem) to new; jump merge] }}>)
+  | _ => ret (false, [i])
+  end.
+
+Definition split_and_merge (c : rctx) (mem : tmem) (i : inst) (acc : list inst) : M (list inst) :=
+  tr <- transform_load_store_inst c mem acc i;;
+  let '(is_split, new_insts) := tr in
+  (* If we split the block in two because of "load"/"store", then all previous instructions *)
+  (* get saved in the new block. New ones stay, and the "merge" lnk gets updated. *)
+  if is_split then
+    ret new_insts
+  (* If we don't split, than we concat new instructions to previous instructions and last "merge" link stays the same *)
+  else
+  (* NOTE: We are folding from the right, so new instructions are appended to the beginning of current block *)
+    ret (new_insts ++ acc).
+
+Definition transform_load_store_blk (c : rctx) (mem : tmem) (nblk : list inst * bool): M (list inst * bool) :=
+  let (bl, is_proc) := nblk in
+  folded <- fold_rightM (split_and_merge c mem) bl <{{ i[ ret ] }}>;;
+  ret (folded, is_proc).
+
+Definition transform_load_store_prog (c : rctx) (mem : tmem) (p : prog) :=
+  let '(p', newp) := mapM (transform_load_store_blk c mem) p (Datatypes.length p) in
+  (p' ++ newp).
+
+(* Example transform := transform_load_store_prog [TPtr; TNum; TPtr]%list [(<{{ i[ ctarget; X := 0; Y <- load[X]; store[Y] <- X] }}>, true)]. 
+Eval compute in transform.
+Eval compute in (Datatypes.length transform).
+Eval compute in (nth_error transform 3). *)
+
+Definition gen_call_wt (c: rctx) (pst: list nat) : G inst :=
+  e <- gen_exp_ptr_wt 1 c pst;;
+  ret <{ call e }>.
+
+Definition _gen_inst_wt (gen_asgn : ty -> rctx -> list nat -> G inst)
+                        (gen_branch : rctx -> nat -> list nat -> nat -> G inst)
+                        (gen_jump : nat -> list nat -> nat -> G inst)
+                        (gen_load : ty -> rctx -> tmem -> nat -> list nat -> G inst)
+                        (gen_store : rctx -> tmem -> nat -> list nat -> G inst)
+                        (gen_call : rctx -> list nat -> G inst)
+                        (c: rctx) (tm: tmem) (sz:nat) (pl: nat) (pst: list nat) : G inst :=
+  let insts := 
+     [ (1, ret ISkip);
+       (1, ret IRet);
+       (sz, t <- arbitrary;; gen_asgn t c pst);
+       (sz, t <- arbitrary;; gen_load t c tm pl pst);
+       (sz, gen_store c tm pl pst);
+       (sz, gen_call c pst) ] in
+  let non_proc_labels := list_minus (seq 0 pl) (proc_hd pst) in
+  match non_proc_labels with
+  | nil => freq_ (ret ISkip) insts
+  | hd :: _ => freq_ (ret ISkip) (insts ++ [ (2, gen_branch c pl pst hd)(* ; (sz, gen_jump pl pst hd) *)])
+  end.
+
+(* redundant functions *)
+Definition gen_nonterm_wt (gen_asgn : ty -> rctx -> list nat -> G inst)
+                          (gen_load : ty -> rctx -> tmem -> nat -> list nat -> G inst)
+                          (gen_store : rctx -> tmem -> nat -> list nat -> G inst)
+                          (gen_call : rctx -> list nat -> G inst)
+                          (c: rctx) (tm: tmem) (sz:nat) (pl: nat) (pst: list nat) : G inst :=
+  freq [ (1, ret ISkip);
+         (sz, t <- arbitrary;; gen_asgn t c pst);
+         (sz, t <- arbitrary;; gen_load t c tm pl pst);
+         (sz, gen_store c tm pl pst);
+         (sz, gen_call c pst)].
+
+Definition _gen_term_wt (gen_branch : rctx -> nat -> list nat -> nat -> G inst)
+                      (gen_jump : nat -> list nat -> nat -> G inst)
+                      (c: rctx) (tm: tmem) (* (sz:nat) *) (pl: nat) (pst: list nat) : G inst :=
+  let non_proc_labels := list_minus (seq 0 pl) (proc_hd pst) in
+  match non_proc_labels with
+  | nil => ret IRet
+  | hd :: _ => freq_ (ret IRet) ([(1, ret IRet) ; (2, gen_jump pl pst hd)])
+  end.
+
+Definition gen_term_wt (c: rctx) (tm: tmem) (pl: nat) (pst: list nat) : G inst :=
+  _gen_term_wt gen_branch_wt gen_jump_wt c tm pl pst.
+
+Definition gen_inst_wt (c: rctx) (tm: tmem) (sz:nat) (pl: nat) (pst: list nat) : G inst :=
+  _gen_inst_wt gen_asgn_wt gen_branch_wt gen_jump_wt gen_load_wt gen_store_wt gen_call_wt
+               c tm sz pl pst.
+
+Definition gen_blk_wt (c: rctx) (tm: tmem) (bsz pl: nat) (pst: list nat) : G (list inst) :=
+  vectorOf bsz (gen_inst_wt c tm bsz pl pst).
+
+Definition _gen_blk_body_wt (c: rctx) (tm: tmem) (bsz pl: nat) (pst: list nat) : G (list inst) :=
+  vectorOf (bsz - 1) (gen_inst_wt c tm bsz pl pst).
+
+Definition gen_blk_with_term_wt (c: rctx) (tm: tmem) (bsz pl: nat) (pst: list nat) : G (list inst) :=
+  blk <- _gen_blk_body_wt c tm bsz pl pst;;
+  term <- gen_term_wt c tm pl pst;;
+  ret (blk ++ [term]).
+
+Definition basic_block_checker (blk: list inst) : bool :=
+  match blk with
+  | [] => false
+  | _ => match seq.last ISkip blk with
+        | IRet | IJump _ => true
+        | _ => false
+        end
+  end.
+
+Definition basic_block_gen_example : G (list inst) :=
+  c <- arbitrary;;
+  tm <- arbitrary;;
+  gen_blk_with_term_wt c tm 8 8 [3; 3; 1; 1].
+
+Definition basic_block_test := (forAll (basic_block_gen_example) (fun (blk: list inst) => (basic_block_checker blk))).
+(*! QuickChick basic_block_test. *)
+
+Fixpoint _gen_proc_with_term_wt (c: rctx) (tm: tmem) (fsz bsz pl: nat) (pst: list nat) : G (list (list inst * bool)) :=
+  match fsz with
+  | O => ret []
+  | S fsz' => n <- choose (1, max 1 bsz);;
+             blk <- gen_blk_with_term_wt c tm n pl pst;;
+             rest <- _gen_proc_with_term_wt c tm fsz' bsz pl pst;;
+             ret ((blk, false) :: rest)
+  end.
+
+Definition gen_proc_with_term_wt (c: rctx) (tm: tmem) (fsz bsz pl: nat) (pst: list nat) : G (list (list inst * bool)) :=
+  match fsz with
+  | O => ret [] (* unreachable *)
+  | S fsz' => n <- choose (1, max 1 bsz);;
+             blk <- gen_blk_with_term_wt c tm n pl pst;;
+             rest <- _gen_proc_with_term_wt c tm fsz' bsz pl pst;;
+             ret ((blk, true) :: rest)
+  end.
+
+Fixpoint _gen_prog_with_term_wt (c: rctx) (tm: tmem) (bsz pl: nat) (pst pst': list nat) : G (list (list inst * bool)) :=
+  match pst' with
+  | [] => ret []
+  | hd :: tl => hd_proc <- gen_proc_with_term_wt c tm hd bsz pl pst;;
+               tl_proc <- _gen_prog_with_term_wt c tm bsz pl pst tl;;
+               ret (hd_proc ++ tl_proc)
+  end.
+
+Definition gen_prog_with_term_wt_example (pl: nat) :=
+  c <- arbitrary;;
+  tm <- arbitrary;;
+  pst <- gen_partition pl;;
+  let bsz := 5%nat in
+  _gen_prog_with_term_wt c tm bsz pl pst pst.
+
+Definition prog_basic_block_checker (p: prog) : bool :=
+  forallb (fun bp => (basic_block_checker (fst bp))) p.
+
+Definition basic_block_wt_test := (forAll (gen_prog_with_term_wt_example 8) (fun (p: prog) => (prog_basic_block_checker p))).
+(*! QuickChick basic_block_wt_test. *)
+
+(* Similarly to "_gen_proc_wf", we generate a procedure with all expressions well-typed (with respect to
+  statuc register context "c : rctx"). Here, "fsz" is the number of blocks in procedure, "bsz" is the
+  number of instructions in the block, and "pl" is the program length. *)
+Fixpoint _gen_proc_wt (c: rctx) (tm: tmem) (psz bsz pl: nat) (pst: list nat) : G (list (list inst * bool)) :=
+  match psz with
+  | O => ret []
+  | S psz' => n <- choose (1, max 1 bsz);;
+             blk <- gen_blk_wt c tm n pl pst;;
+             rest <- _gen_proc_wt c tm psz' bsz pl pst;;
+             ret ((blk, false) :: rest)
+  end.
+
+Definition gen_proc_wt (c: rctx) (tm: tmem) (psz bsz pl: nat) (pst: list nat) : G (list (list inst * bool)) :=
+  match psz with
+  | O => ret [] (* unreachable *)
+  | S psz' => n <- choose (1, max 1 bsz);;
+             blk <- gen_blk_wt c tm n pl pst;;
+             rest <- _gen_proc_wt c tm psz' bsz pl pst;;
+             ret ((blk, true) :: rest)
+  end.
+
+Fixpoint _gen_prog_wt (c: rctx) (tm: tmem) (bsz pl: nat) (pst pst': list nat) : G (list (list inst * bool)) :=
+  match pst' with
+  | [] => ret []
+  | hd :: tl => hd_proc <- gen_proc_wt c tm hd bsz pl pst;;
+               tl_proc <- _gen_prog_wt c tm bsz pl pst tl;;
+               ret (hd_proc ++ tl_proc)
+  end.
+
+Definition gen_prog_wt_example (pl: nat) :=
+  c <- arbitrary;;
+  tm <- arbitrary;;
+  pst <- gen_partition pl;;
+  let bsz := 5%nat in
+  _gen_prog_wt c tm bsz pl pst pst.
+
+Definition test_wt_example : G bool :=
+  prog <- gen_prog_wt_example 8;;
+  ret (wf prog).
+
+Definition gen_prog_wt (bsz pl: nat) :=
+  c <- arbitrary;;
+  tm <- arbitrary;;
+  pst <- gen_partition pl;;
+  _gen_prog_wt c tm bsz pl pst pst.
+
+Definition gen_prog_wt' (c : rctx) (pst : list nat) (bsz pl : nat) :=
+  tm <- arbitrary;;
+  _gen_prog_wt c tm bsz pl pst pst.
+
+Definition wt_wf := (forAll (gen_prog_wt 3 8) (fun (p : prog) => (wf p))).
+(*! QuickChick wt_wf. *)
+Definition wt_uslh_wf := (forAll (gen_prog_wt 3 8) (fun (p : prog) => (wf (uslh_prog p)))).
+(*! QuickChick wt_uslh_wf. *)
+
+(* The well-typed expression "always evaluates" in the register set produces by "gen_reg_wt " *)
+Definition wt_expr_is_defined := (
+    forAll arbitrary (fun (c : rctx) =>
+    forAll arbitrary (fun (pl : nat) =>
+    forAll (choose (2, 5)) (fun (exp_sz : nat) => 
+    pst <- gen_partition pl;;
+    forAll (gen_reg_wt c pst) (fun (r : reg) =>
+    forAll (gen_exp_wt exp_sz c pst) (fun (e : exp) =>
+    is_defined (eval r e)
+  )))))).
+(*! QuickChick wt_expr_is_defined. *)
+
+(* "+++ Passed 10000 tests (0 discards)" *)
+
+(* To evaluate our generator, we proceed by creating a predicate, which checks kind of type checks the
+  program. *)
+
+Fixpoint ty_exp (c: rctx) (e: exp) : option ty :=
+  match e with
+  | ANum _ => Some TNum
+  | FPtr _ => Some TPtr
+  | AId x => Some (t_apply c x)
+  | ACTIf e1 e2 e3 => match ty_exp c e1 with
+                     | Some TNum => match ty_exp c e2, ty_exp c e3 with
+                                   | Some TNum, Some TNum => Some TNum
+                                   | Some TPtr, Some TPtr => Some TPtr
+                                   | _, _ => None
+                                   end
+                     | _ => None
+                     end
+  | ABin bop e1 e2 => match bop with
+                     | BinEq =>  match ty_exp c e1, ty_exp c e2 with
+                                | Some t1, Some t2 => if (ty_eqb t1 t2) then Some TNum else None
+                                | _, _ => None
+                                end
+                     | _ => match ty_exp c e1, ty_exp c e2 with
+                           | Some TNum, Some TNum => Some TNum
+                           | _, _ => None
+                           end
+                     end
+  end.
+
+(* The "ty_inst" predicate checks if the instruction "i" in the program "p" is well-typed with respect to
+  register context "c" and a typed memory "tm". *)
+Fixpoint ty_inst (c: rctx) (tm: tmem) (p: prog) (i: inst) : bool :=
+  match i with
+  | ISkip | ICTarget | IRet => true
+  | IAsgn x e => match ty_exp c e with
+                | Some t => ty_eqb (t_apply c x) t
+                | _ => false
+                end
+  | IBranch e l => match ty_exp c e with
+                  | Some TNum => wf_label p false l
+                  | _ => false
+                  end
+  | IJump l => wf_label p false l
+  (* let's trust generator. *)
+  | ILoad x e => match e with
+                | ANum n =>
+                    match nth_error tm n with
+                    | Some t => ty_eqb (t_apply c x) t
+                    | _ => false
+                    end
+                | _ => match ty_exp c e with
+                      | Some TNum => true
+                      | _ => false
+                      end
+                end
+  | IStore a e => match a with
+                 | ANum n =>
+                     match nth_error tm n, ty_exp c e with
+                     | Some t1, Some t2 => ty_eqb t1 t2
+                     | _, _ => false
+                     end
+                 | _ => match ty_exp c a, ty_exp c e with
+                       | Some TNum, Some _ => true
+                       | _, _ => false
+                       end
+                 end
+  | ICall e => match e with
+              | FPtr l => wf_label p true l
+              | _ => match ty_exp c e with
+                    | Some TPtr => true
+                    | _ => false
+                    end
+              end
+  end.
+
+Definition ty_blk (c: rctx) (tm: tmem) (p: prog) (blk: list inst * bool) : bool :=
+  forallb (ty_inst c tm p) (fst blk).
+
+Definition ty_prog (c: rctx) (tm: tmem) (p: prog) : bool :=
+  forallb (ty_blk c tm p) p.
+
+Definition gen_prog_ty_ctx_wt (bsz pl: nat) : G (rctx * tmem * prog) :=
+  c <- arbitrary;;
+  tm <- arbitrary;;
+  pst <- gen_partition pl;;
+  p <- _gen_prog_wt c tm bsz pl pst pst;;
+  ret (c, tm, p).
+
+Definition ty_prog_wf := (forAll (gen_prog_ty_ctx_wt 3 8) (fun '(c, tm, p) => ((ty_prog c tm p) && (wf p)))).
+
+(** Relative Security *)
+
+(* Taint Tracker for input pairs *)
+
+Definition join (l1 l2 : label) : label := l1 && l2.
+
+Fixpoint vars_exp (e:exp) : list string :=
+  match e with
+  | ANum n => []
+  | AId i => [i]
+  | ABin op e1 e2 => vars_exp e1 ++ vars_exp e2
+  | ACTIf e1 e2 e3 => vars_exp e1 ++ vars_exp e2 ++ vars_exp e3
+  | FPtr n => []
+  end.
+
+Definition vars_inst (i: inst) : list string :=
+  match i with
+  | ISkip | IRet | ICTarget | IJump _ => []
+  | IAsgn x e => x :: vars_exp e
+  | IBranch e l => vars_exp e
+  | ILoad x e => x :: vars_exp e
+  | IStore e1 e2 => vars_exp e1 ++ vars_exp e2
+  | ICall e => vars_exp e
+  end.
+
+Fixpoint vars_blk (blk: list inst) : list string :=
+  List.concat (map vars_inst blk).
+
+Fixpoint _vars_prog (p: prog) : list string :=
+  match p with
+  | [] => []
+  | (blk, _) :: tl => vars_blk blk ++ _vars_prog tl
+  end.
+
+Definition vars_prog (p: prog) : list string :=
+  remove_dupes String.eqb (_vars_prog p).
+
+Definition label_of_exp (P:pub_vars) (e:exp) : label :=
+  List.fold_left (fun l a => join l (P ! a)) (vars_exp e) public.
+
+(* Copied from TestingFlexSLH.v *)
+
+(** Some generators *)
+
+Definition gen_prog_ty_ctx_wt' (bsz pl: nat) : G (rctx * tmem * list nat * prog) :=
+  c <- arbitrary;;
+  tm <- arbitrary;;
+  pst <- gen_partition pl;;
+  p <- _gen_prog_wt c tm bsz pl pst pst;;
+  ret (c, tm, pst, p).
+
+Definition gen_prog_wt_with_basic_blk (bsz pl: nat) : G (rctx * tmem * list nat * prog) :=
+  c <- arbitrary;;
+  tm <- arbitrary;;
+  pst <- gen_partition pl;;
+  p <- _gen_prog_with_term_wt c tm bsz pl pst pst;;
+  ret (c, tm, pst, p).
+
+Definition gen_wt_mem (tm: tmem) (pst: list nat) : G mem :=
+  let indices := seq 0 (Datatypes.length tm) in
+  let idx_tm := combine indices tm in
+  let gen_binds := mapGen (fun '(idx, t) => (v <- gen_val_wt t pst;; ret (idx, v))) idx_tm in
+  r <- gen_binds;;
+  ret (snd (split r)).
+
+(** Some common definitions *)
+
+Definition ipc : cptr := (0 , 0).
+Definition istk : list cptr := [].
+Definition all_possible_vars : list string := (["X0"%string; "X1"%string; "X2"%string; "X3"%string; "X4"%string; "X5"%string]).
+
+Fixpoint member (n: nat) (l: list nat) : bool :=
+  match l with
+  | [] => false
+  | hd::tl => if (hd =? n) then true else member n tl
+  end.
+
+Fixpoint _tms_to_pm (tms: list nat) (len: nat) (cur: nat) : list label :=
+  match len with
+  | 0 => []
+  | S len' => member cur tms :: _tms_to_pm tms len' (S cur)
+  end.
+
+(* Calculate public memory from taint memory *)
+Definition tms_to_pm (len: nat) (tms: list nat) : list label :=
+  _tms_to_pm tms len 0.
+
+Compute (tms_to_pm 8 [3; 4; 5]).
+
+(* well-type checkers *)
+Definition wt_valb (v: val) (t: ty) : bool :=
+  match v, t with
+  | N _, TNum | FP _, TPtr => true
+  | _, _ => false
+  end.
+
+Definition rs_wtb (rs : total_map val) (c : rctx) : bool :=
+  let '(dv, m) := rs in
+  let '(dt, tm) := c in
+  wt_valb dv dt && forallb (fun '(x, t) => wt_valb (t_apply rs x) t) tm.
+
+Fixpoint _gen_pub_mem_equiv_same_ty (P : list label) (m: list val) : G (list val) :=
+  let f := fun v => match v with
+                 | N _ => n <- arbitrary;; ret (N n)
+                 | FP _ => l <- arbitrary;; ret (FP l)
+                 | UV => ret UV (* shouldn't happen *)
+                 end in
+  match P, m with
+  | [], [] => ret []
+  | hdp::tlp, hdm::tlm =>
+      hd <- (if hdp then ret hdm else f hdm);;
+      tl <-_gen_pub_mem_equiv_same_ty tlp tlm;;
+      ret (hd::tl)
+  | _, _ => ret [] (* unreachable *)
+  end.
+
+Fixpoint gen_pub_mem_equiv_same_ty (P : list label) (m: list val) : G (list val) :=
+  if (Datatypes.length P =? Datatypes.length m)
+  then _gen_pub_mem_equiv_same_ty P m
+  else ret [].
+
+Definition m_wtb (m: mem) (tm: tmem) : bool :=
+  let mtm := combine m tm in
+  forallb (fun '(v, t) => wt_valb v t) mtm.
+
+(* check 2: no observation -> no leaked *)
+
+Definition gen_inst_no_obs (pl: nat) (pst: list nat) : G inst :=
+  let jlb := (list_minus (seq 0 (pl - 1)) (proc_hd pst)) in
+  if seq.nilp jlb
+  then ret <{ skip }>
+  else freq [
+           (1, ret ISkip);
+           (1, ret IRet);
+           (1, l <- elems_ 0 jlb;; ret (IJump l))
+         ].
+
+Definition gen_blk_no_obs (bsz pl: nat) (pst: list nat) : G (list inst) :=
+  vectorOf bsz (gen_inst_no_obs pl pst).
+
+Fixpoint _gen_proc_no_obs (fsz bsz pl: nat) (pst: list nat) : G (list (list inst * bool)) :=
+  match fsz with
+  | O => ret []
+  | S fsz' =>
+      n <- choose (1, max 1 bsz);;
+      blk <- gen_blk_no_obs n pl pst;;
+      rest <- _gen_proc_no_obs fsz' bsz pl pst;;
+      ret ((blk, false) :: rest)
+  end.
+
+Definition gen_proc_no_obs (fsz bsz pl: nat) (pst: list nat) : G (list (list inst * bool)) :=
+  match fsz with
+  | O => ret []
+  | S fsz' =>
+      n <- choose (1, max 1 bsz);;
+      blk <- gen_blk_no_obs n pl pst;;
+      rest <- _gen_proc_no_obs fsz' bsz pl pst;;
+      ret ((blk, true) :: rest)
+  end.
+
+Fixpoint _gen_prog_no_obs (bsz pl: nat) (pst pst': list nat) : G (list (list inst * bool)) :=
+  match pst' with
+  | [] => ret []
+  | hd :: tl =>
+      hd_proc <- gen_proc_no_obs hd bsz pl pst;;
+      tl_proc <- _gen_prog_no_obs bsz pl pst tl;;
+      ret (hd_proc ++ tl_proc)
+  end.
+
+Definition gen_no_obs_prog : G prog :=
+  pl <- choose(2, 6);; (* Generate small but non-trivial programs *)
+  pst <- gen_partition pl;;
+  let bsz := 3 in (* Max instructions per block *)
+  _gen_prog_no_obs bsz pl pst pst.
+
+Definition empty_mem : mem := [].
+
+Definition empty_rs : reg := t_empty (FP 0).
+
+(** Tests for Speculative Execution *)
+
+Derive Show for direction.
+Derive Show for observation.
+
+Definition spec_rs (rs: reg) := (callee !-> (FP 0); (msf !-> (N 0); rs)).
+
+(* ** Direction generators *)
+
+Definition gen_dbr : G direction :=
+  b <- arbitrary;; ret (DBranch b).
+
+Definition gen_dcall (pst: list nat) : G direction :=
+  l <- (elems_ 0 (proc_hd pst));; ret (DCall (l, 0)).
+
+Variant sc_output_st : Type :=
+  | SRStep : obs -> dirs -> spec_cfg -> sc_output_st
+  | SRError : obs -> dirs -> spec_cfg -> sc_output_st
+  | SRTerm : obs -> dirs -> spec_cfg -> sc_output_st.
+
+Definition gen_step_direction (i: inst) (c: cfg) (pst: list nat) : G dirs :=
+  let '(pc, rs, m, s) := c in
+  match i with
+  | <{ branch e to l }> => db <- gen_dbr;; ret [db]
+  | <{ call e }> =>  dc <- gen_dcall pst;; ret [dc]
+  | _ => ret []
+  end.
+
+Definition gen_spec_step (p:prog) (sc:spec_cfg) (pst: list nat) : G sc_output_st :=
+  let '(c, ct, ms) := sc in
+  let '(pc, r, m, sk) := c in
+  match p[[pc]] with
+  | Some i =>
+      match i with
+      | <{{branch e to l}}> =>
+          d <- gen_dbr;;
+          ret (match spec_step p (S_Running sc) [d] with
+               | (S_Running sc', dir', os') => SRStep os' [d] sc'
+               | _ => SRError [] [] sc
+               end)
+      | <{{call e}}> =>
+          d <- gen_dcall pst;;
+          ret (match spec_step p (S_Running sc) [d] with
+               | (S_Running sc', dir', os') => SRStep os' [d] sc'
+               | _ => SRError [] [] sc
+               end)
+      | IRet | ICTarget =>
+          ret (match spec_step p (S_Running sc) [] with
+               | (S_Running sc', dir', os') => SRStep os' [ ] sc'
+               | (S_Term, _, _) => SRTerm [] [] sc
+               | _ => SRError [] [] sc
+               end)
+      | _ =>
+          ret (match spec_step p (S_Running sc) [] with
+               | (S_Running sc', dir', os') => SRStep os' [ ] sc'
+               | _ => SRError [] [] sc
+               end)
+      end
+  | None => ret (SRError [] [] sc)
+  end.
+
+Variant spec_exec_result : Type :=
+  | SETerm (sc: spec_cfg) (os: obs) (ds: dirs)
+  | SEError (sc: spec_cfg) (os: obs) (ds: dirs)
+  | SEOutOfFuel (sc: spec_cfg) (os: obs) (ds: dirs).
+
+#[export] Instance showSER : Show spec_exec_result :=
+  {show :=fun ser => 
+      match ser with
+      | SETerm sc os ds => show ds
+      | SEError _ _ ds => ("error!!"%string ++ show ds)%string
+      | SEOutOfFuel _ _ ds => ("oof!!"%string ++ show ds)%string
+      end
+  }.
+
+Fixpoint _gen_spec_steps_sized (f : nat) (p:prog) (pst: list nat) (sc:spec_cfg) (os: obs) (ds: dirs) : G (spec_exec_result) :=
+  match f with
+  | 0 => ret (SEOutOfFuel sc os ds)
+  | S f' =>
+      sr <- gen_spec_step p sc pst;;
+      match sr with
+      | SRStep os1 ds1 sc1 =>
+          _gen_spec_steps_sized f' p pst sc1 (os ++ os1) (ds ++ ds1)
+      | SRError os1 ds1 sc1 =>
+          (* trace ("ERROR STATE: " ++ show sc1)%string *)
+          (ret (SEError sc1 (os ++ os1) (ds ++ ds1)))
+      | SRTerm  os1 ds1 sc1 =>
+          ret (SETerm sc1 (os ++ os1) (ds ++ ds1))
+      end
+  end.
+
+Definition gen_spec_steps_sized (f : nat) (p:prog) (pst: list nat) (sc:spec_cfg) : G (spec_exec_result) :=
+  _gen_spec_steps_sized f p pst sc [] [].
+
+(* Speculative Step functions *)
+Definition spec_step_acc (p:prog) (sc:spec_cfg) (ds: dirs) : sc_output_st :=
+  match spec_step p (S_Running sc) ds with
+  | (S_Running sc', ds', os) => SRStep os ds' sc' (* sc': current spec_cfg, os: observations, ds': remaining dirs *)
+  | (S_Term, _, _) => SRTerm [] [] sc
+  | _ => SRError [] [] sc
+  end.
+
+Fixpoint _spec_steps_acc (f : nat) (p:prog) (sc:spec_cfg) (os: obs) (ds: dirs) : spec_exec_result :=
+  match f with
+  | 0 => SEOutOfFuel sc os ds (* sc: current spec_cfg, os: observations, ds: remaining dirs *)
+  | S f' =>
+      match spec_step_acc p sc ds with
+      | SRStep os1 ds1 sc1 =>
+          _spec_steps_acc f' p sc1 (os ++ os1) ds1
+      | SRError os1 ds1 sc1 =>
+          (SEError sc1 (os ++ os1) ds1)
+      | SRTerm os1 ds1 sc1 =>
+          (SETerm sc1 (os ++ os1) ds1)
+      end
+  end.
+
+Definition spec_steps_acc (f : nat) (p:prog) (sc:spec_cfg) (ds: dirs) : spec_exec_result :=
+  _spec_steps_acc f p sc [] ds.
