TaintTrackingMiniCET.v
@@ -1,0 +1,245 @@
+Set Warnings "-notation-overridden,-parsing,-deprecated-hint-without-locality".
+From Stdlib Require Import Strings.String.
+From SECF Require Import Maps.
+From Stdlib Require Import Bool.Bool.
+From Stdlib Require Import Arith.Arith.
+From Stdlib Require Import Arith.EqNat.
+From Stdlib Require Import Arith.PeanoNat.
+From Stdlib Require Import Lia.
+From Stdlib Require Import List. Import ListNotations.
+Set Default Goal Selector "!".
+
+From QuickChick Require Import QuickChick Tactics.
+Import QcNotation QcDefaultNotation. Open Scope qc_scope.
+Require Export ExtLib.Structures.Monads.
+Require Import ExtLib.Data.List.
+Import MonadNotation.
+From Stdlib Require Import String.
+From SECF Require Import ListMaps MapsFunctor MiniCET Utils.
+Require Import Stdlib.Classes.EquivDec.
+
+(* For testing relative security we do taint tracking of sequential executions
+   (as a variant of Lucie's interpreter). We use this to track which initial
+   values of variables and arrays affect CT observations. *)
+Notation t_apply := ListTotalMap.t_apply.
+
+Definition reg_id := string.
+Definition mem_addr := nat.
+
+Definition taint : Type := list (reg_id + mem_addr).
+
+#[export] Instance showTaint : Show (reg_id + mem_addr) :=
+  {show := fun x =>
+     match x with
+     | inl x => show x
+     | inr a => show a
+     end}.
+
+Definition sum_eqb (s1 s2 : (reg_id + mem_addr)) : bool :=
+  match s1, s2 with
+  | inl x1, inl x2 => String.eqb x1 x2
+  | inr x1, inr x2 => Nat.eqb x1 x2
+  | _, _ => false
+  end.
+
+Definition join_taints t1 t2 := remove_dupes sum_eqb (t1 ++ t2).
+
+Module TaintTracking (ST: Semantics).
+
+Definition tcptr := taint.
+Definition treg := ListTotalMap.t taint.
+Definition tamem := list taint.
+Definition tstk := list tcptr.
+
+Definition tcfg := (tcptr * treg * tamem * tstk)%type.
+Definition input_st : Type := ST.cfg * tcfg * taint.
+
+(* Currently, we generate UB-free programs based on abstract states.
+   Going forward, we'll transition to execution-based program
+   generation, which also produces UB-free programs. Therefore,
+   we don't need to worry about UB in either case. *)
+
+Variant output_st (A : Type) : Type :=
+  | RStep : A -> obs -> input_st -> output_st A
+  | RError : obs -> input_st -> output_st A
+  | RTerm : obs -> input_st -> output_st A.
+
+Record evaluator (A : Type) : Type := mkEvaluator
+  { evaluate : input_st -> output_st A }.
+
+(* An 'evaluator A'. This is the monad.
+   It transforms an input state into an output state, returning an A. *)
+(* An interpreter is a special kind of evaluator *)
+Definition interpreter: Type := evaluator unit.
+
+(* Generic monad operators *)
+#[export] Instance monadEvaluator: Monad evaluator :=
+  { ret := fun A value => mkEvaluator A (fun (ist : input_st) => RStep A value [] ist);
+    bind := fun A B e f =>
+      mkEvaluator B (fun (ist : input_st) =>
+        match evaluate A e ist with
+        | RStep _ value os1 ist'  =>
+            match evaluate B (f value) ist' with
+            | RStep _ value os2 ist'' => RStep B value (os1 ++ os2) ist''
+            | RError _ os2 ist'' => RError B (os1 ++ os2) ist''
+            | RTerm _ os2 ist'' => RTerm B (os1 ++ os2) ist''
+            end
+        | RError _ os ist' => RError B os ist'
+        | RTerm _ os ist' => RTerm B os ist'
+        end
+      )
+  }.
+
+Fixpoint _calc_taint_exp (e: exp) (tr: treg) : taint :=
+  match e with
+  | ANum _ | FPtr _ => []
+  | AId x => t_apply tr x
+  | ABin _ e1 e2 => join_taints (_calc_taint_exp e1 tr) (_calc_taint_exp e2 tr)
+  | ACTIf e1 e2 e3 => join_taints (_calc_taint_exp e1 tr)
+                                 (join_taints (_calc_taint_exp e2 tr) (_calc_taint_exp e3 tr))
+  end.
+
+Variant taint_ctx :=
+  | CMem (n: nat)
+  | CDefault.
+
+(* None cases are unreachable. *)
+Definition taint_step (i: inst) (c: ST.cfg) (tc: tcfg) (tobs: taint) (tctx: taint_ctx) : option (tcfg * taint) :=
+  let '(pc, rs, m, s) := c in
+  let '(tpc, trs, tm, ts) := tc in
+  match i with
+  | <{ skip }> | <{ ctarget }> | <{ jump _ }> =>
+      match tctx with
+      | CDefault => Some (tc, tobs)
+      | _ => None
+      end
+  | <{ x := e }> =>
+      match tctx with
+      | CDefault =>
+          let te := (_calc_taint_exp e trs) in
+          let tx := join_taints te tpc in
+          let tc' := (tpc, (x !-> tx; trs), tm, ts) in
+          Some (tc', tobs)
+      | _ => None
+      end
+  | <{ branch e to l }> =>
+      match tctx with
+      | CDefault =>
+          let te := (_calc_taint_exp e trs) in
+          let tpc' := join_taints te tpc in
+          let tc' := (tpc', trs, tm, ts) in
+          let tobs' := join_taints tobs tpc' in
+          Some (tc', tobs')
+      | _ => None
+      end
+  | <{ x <- load[e] }> =>
+      match tctx with
+      | CMem n =>
+          let te := (_calc_taint_exp e trs) in
+          let tv := nth n tm [] in (* default case is unreachable: step already checked. *)
+          let tx := (join_taints (join_taints te tv) tpc) in
+          let tc' := (tpc, (x !-> tx; trs), tm, ts) in
+          let tobs' := (join_taints (join_taints te tpc) tobs) in
+          Some (tc', tobs')
+      | _ => None
+      end
+  | <{ store[e] <- e' }> =>
+      match tctx with
+      | CMem n =>
+          let te := (_calc_taint_exp e trs) in
+          let te' := (_calc_taint_exp e' trs) in
+          let tm_val := join_taints (join_taints te te') tpc in
+          let tc' := (tpc, trs, upd n tm tm_val, ts) in
+          let tobs' := join_taints (join_taints te tpc) tobs in
+          Some (tc', tobs')
+      | _ => None
+      end
+  | <{ call e }> =>
+      match tctx with
+      | CDefault =>
+          let te := (_calc_taint_exp e trs) in
+          let ts' := tpc :: ts in
+          let tpc' := join_taints te tpc in
+          let tc' := (tpc', trs, tm, ts') in
+          let tobs' := join_taints tobs tpc' in
+          Some (tc', tobs')
+      | _ => None
+      end
+  | <{ ret }> =>
+      match tctx with
+      | CDefault =>
+          let tpc' := hd [] ts in (* default case is unreachable: step already checked. *)
+          let ts' := tl ts in
+          let tc' := (tpc', trs, tm, ts') in
+          Some (tc', tobs)
+      | _ => None
+      end
+  end.
+
+Definition get_ctx (rs: ST.REG) (i: inst) : option taint_ctx  :=
+  match i with
+  | <{ x <- load[e] }> => n <- to_nat (ST.eval rs e);;
+                        Some (CMem n)
+  | <{ store[e] <- e' }> => n <- to_nat (ST.eval rs e);;
+                          Some (CMem n)
+  | _ => Some CDefault
+  end.
+
+(* ret with empty stackframe *)
+Definition final_cfg (p: prog) (c: ST.cfg) : bool :=
+  let '(pc, rs, m, stk) := c in
+  match ST.fetch p pc with
+  | Some i => match i with
+             | IRet => if seq.nilp stk then true else false (* Normal Termination *)
+             | _ => false
+             end
+  | None => false
+  end.
+
+Definition step_taint_track (p: prog) : evaluator unit :=
+  mkEvaluator _ (fun (ist : input_st) =>
+    let '(c, tc, tobs) := ist in
+    let '(pc, rs, m, s) := c in
+    let '(tpc, trs, tm, ts) := tc in
+    match ST.step p (S_Running c) with
+    | (S_Running c', os) =>
+        match (ST.fetch p pc) with
+        | Some i => match get_ctx rs i with
+                   | Some tctx => match taint_step i c tc tobs tctx with
+                                 | Some (tc', tobs') => RStep _ tt os (c', tc', tobs')
+                                 | _ => RError _ [] ist (* context is inconsistent. *)
+                                 end
+                   | _ => RError _ [] ist (* For now, unreachable *)
+                   end
+        | _ => RError _ [] ist
+        end
+    | (S_Term, []) => RTerm _ [] ist
+    | _ => RError _ [] ist
+    end).
+
+Variant exec_result : Type :=
+  | ETerm (st: input_st) (os: obs)
+  | EError (st: input_st) (os: obs)
+  | EOutOfFuel (st: input_st) (os: obs).
+
+Fixpoint steps_taint_track (f: nat) (p: prog) (ist: input_st) (os: obs) : exec_result :=
+  match f with
+  | O => EOutOfFuel ist os
+  | S f' =>
+      match evaluate unit (step_taint_track p) ist with
+      | RTerm _ os' ist' => ETerm ist' (os ++ os')
+      | RError _ os' ist' => EError ist' (os ++ os')
+      | RStep _ _ os' ist' => steps_taint_track f' p ist' (os ++ os')
+      end
+  end.
+
+Fixpoint _init_taint_mem (m: mem) (n: nat) : tamem :=
+  match m with
+  | [] => []
+  | h :: m' => ([inr n]) :: _init_taint_mem m' (S n)
+  end.
+
+Definition init_taint_mem (m: mem) : tamem :=
+  _init_taint_mem m 0.
+
+End TaintTracking.
